\documentclass[fleqn,a4paper]{scrartcl}

\usepackage{fullpage}
\usepackage[utf8]{inputenc}
\usepackage{lmodern}
\usepackage{amsmath}
\usepackage{amssymb}
\usepackage{amsfonts}
\usepackage{pgfplots}
\usepackage{tikz}
\usepackage{pgf}

\begin{document}
%start
Bsp 2) \\\\ {\large $ \int x \cos x dx $ }
\begin{eqnarray*}
u' =& \cos x \Rightarrow u &= \sin x \\
v =& x \quad \Rightarrow \quad v' &= 1 
\end{eqnarray*}
$
\int x \cos x dx = x \sin x - \int 1*\sin x dx $ \\$
= x \sin x + \cos x + c
$ \\\\ Bsp 3)\\\\ {\large $ I = \int x^n \sin x dx $  }
\begin{eqnarray*}
u' =& \sin x \Rightarrow u &= -\cos x \\
v =& x^n \Rightarrow v' &= n x^{n-1}
\end{eqnarray*}
$
I= -x^n \cos x - \int - ux^{n -1}  \cos x dx = -x^n \cos x + n \int x^{n-1} \cos x dx$ \\\\ iterativ mittels partieller Integration den Grad von $ x^n$ um $ 1 $ vermindern \\\\$
\int x^2 \sin x dx 
$
\begin{eqnarray*}
u' =& \sin x \qquad u &= -cos x \\
v =& x^2 \qquad v' &= 2x
\end{eqnarray*}
$
\int x^2 \sin x dx = -x^2 \cos x - \int 2x (-\cos x) dx$ \\ 
\begin{eqnarray*}
=& -x^2 \cos x +2 \int x \cos x dx \\
=& -x^2 \cos x + 2 (x \sin x + \cos x) +c \\
=& (2 - x^2) \cos x + 2 x \sin x +c
\end{eqnarray*}
Bsp 4) \\\\
$ \int \sin^2 x dx $ \\ 
\begin{eqnarray*}
u' =& \sin x \Rightarrow u &= -\cos x \\
v =& \sin x \Rightarrow v' &= \cos x
\end{eqnarray*}
\begin{eqnarray*}
I =& \int \sin^2 x dx = - \sin x \cos x - \int - \cos^2 x dx \\
=& -\sin x \cos x + \int \cos^2 x dx \\
=& -\sin x \cos x + \int (1-\sin^2 x) dx \\
=& -\sin \cos x + \int dx - \int \sin^2 x dx \\
=& -\sin \cos x + x- \int \sin^2 x dx \\
=& -\sin x \cos x + x - I \vert + I
2 I=& - \sin x \cos x + x + 2c \\
I =& - \frac{1}{2} \sin x \cos x + \frac{x}{2} +c \\ 
\end{eqnarray*}
\underline{Berechnen von bestimmten Integralen} \\\\
mittels partieller Integration \\\\
$\int\limits_a^b u'(x) v(x) dx = u(x) v (x)\underset{b}{\overset{a}{ \bigg{ \vert}}} - \int\limits_a^b u (x) v'(x) dx $ \\\\\\ Bsp $
\int\limits_0^2 x e^x dx = x e^x \underset{0}{\overset{2}{ \bigg{ \vert}}} - \int\limits_0^2 e^x dx $ \\ 
\begin{eqnarray*}
u' =& e^x \Rightarrow u &= e^x \\
v =& x \Rightarrow v' &= 1 
\end{eqnarray*}
$
=[xe^x-e^x\underset{0}{\overset{3}{]}} = (x-1)e^x \underset{0}{\overset{2}{ \bigg{ \vert}}} = \underbrace{e^2}_{2} - \underbrace{(e^0)}_{0} = e^2 +1
$
%stop
\end{document}